

3.8

3-5. 解:

$$(1) \quad y''(t) + 3y'(t) + 2y(t) = f(t), t > 0; \quad f(t) = u(t) \quad y(0^+) = 1, y'(0^+) = 1$$

$$\text{齐次方程为 } y''(t) + 3y'(t) + 2y(t) = 0 \quad \text{特征方程 } \lambda^2 + 3\lambda + 2 = 0$$

固有响应 特征根  $\lambda_1 = -1, \lambda_2 = -2$ 

$$\text{齐次解 } y_h(t) = Ae^{-t} + Be^{-2t}$$

$$f(t) = u(t) \quad \text{令 } y_p(t) = C \quad (t > 0)$$

$$\text{强迫响应 } y_p(t) = C$$

$$\text{完全解 } y(t) = Ae^{-t} + Be^{-2t} + C, \text{ 代入原式}$$

$$\therefore C = 1$$

$$y(0^+) = A + B + 1 = 1 \quad y'(0^+) = -A - 2B = 1$$

$$\therefore A = -1, B = -1$$

$$\text{固有响应 } y_h(t) = e^{-t} + e^{-2t}, \text{ 强迫响应 } y_p(t) = 1$$

$$\text{完全响应 } y(t) = -e^{-t} + e^{-2t} + 1$$

$$(2) \quad y''(t) + 3y'(t) + 2y(t) = 2f(t) \quad f(t) = \cos 2t \cdot u(t) \quad y(0^+) = 1 \quad y'(0^+) = 1$$

$$\text{由 (1) 可知, 固有响应 } y_h(t) = Ae^{-t} + Be^{-2t}$$

$$\text{受迫响应 } y_p(t) = C \cos 2t + D \sin 2t \quad \text{代入原式可得} \quad \begin{cases} C = -\frac{1}{10} \\ D = \frac{3}{10} \end{cases}$$

$$\therefore \text{完全响应 } y(t) = Ae^{-t} + Be^{-2t} - \frac{1}{10} \cos 2t + \frac{3}{10} \sin 2t \quad (t > 0)$$

$$y(0^+) = A + B - \frac{1}{10} = 1$$

$$y'(0^+) = -A - 2B + \frac{3}{5} = 1 \quad \Rightarrow \quad A = -\frac{3}{2}, B = \frac{13}{5}$$

$$\therefore \text{自固有响应 } y_h(t) = -\frac{3}{2}e^{-t} + \frac{13}{5}e^{-2t}$$

$$\text{受迫响应 } y_p(t) = -\frac{1}{10} \cos 2t + \frac{3}{10} \sin 2t$$

$$\text{完全响应 } y(t) = -\frac{3}{2}e^{-t} + \frac{13}{5}e^{-2t} - \frac{1}{10} \cos 2t + \frac{3}{10} \sin 2t$$



(3)  $y''(t) + 4y'(t) + 2y(t) = f(t)$ ,  $t > 0$ ;  $f(t) = e^{-t}u(t)$ ,  $y(0^+) = 1$ ,  $y'(0^+) = 1$   
 齐次方程  $y''(t) + 4y'(t) + 2y(t) = 0$

特征根  $\alpha_1 = -2 + \sqrt{2}$ ,  $\alpha_2 = -2 - \sqrt{2}$

固有响应  $y_h(t) = Ae^{(-2+\sqrt{2})t} + Be^{(-2-\sqrt{2})t}$

受迫响应  $y_p(t) = Ce^{-t}$  ( $t > 0$ ) 代入可得  $C = -1$

完全响应  $y(t) = Ae^{(-2+\sqrt{2})t} + Be^{(-2-\sqrt{2})t} + e^{-t}$

$y(0^+) = A + B + 1 = 1$   $y'(0^+) = (-2+\sqrt{2})A + (-2-\sqrt{2})B - 1 = 1$

$\therefore A = \frac{\sqrt{2}}{2}$ ,  $B = -\frac{\sqrt{2}}{2}$

固有响应  $y_h(t) = \frac{\sqrt{2}}{2}e^{(-2+\sqrt{2})t} - \frac{\sqrt{2}}{2}e^{(-2-\sqrt{2})t}$

受迫响应  $y_p(t) = -e^{-t}$

完全响应  $y(t) = \frac{\sqrt{2}}{2}e^{(-2+\sqrt{2})t} - \frac{\sqrt{2}}{2}e^{(-2-\sqrt{2})t} - e^{-t}$  ( $t > 0$ )

3-4. 解:  $y'(t) + 3y(t) = f(t)$  ( $t > 0$ )

齐次方程:  $y'(t) + 3y(t) = 0$

特征根  $\alpha = -3$

$\therefore$  固有响应  $y_h(t) = Ae^{-3t}$

(1)  $f(t) = u(t)$   $\therefore y_p(t) = B$ ,  $y(t) = Ae^{-3t} + B$

$\therefore \begin{cases} 3B = 1 \\ y(0^+) = A + B = 1 \end{cases} \Rightarrow A = \frac{2}{3}, B = \frac{1}{3}$

固有响应  $y_h(t) = \frac{2}{3}e^{-3t}$ ,  $y_p(t) = \frac{1}{3}$   $y(t) = \frac{2}{3}e^{-3t} + \frac{1}{3}$  ( $t > 0$ )

(2)  $f(t) = e^{-t}u(t)$ ,  $y_p(t) = Be^{-t}$ , 代入  $y(t) = Ae^{-3t} + Be^{-t}$

$\therefore \begin{cases} 2B = 1 \\ A + B = 1 \end{cases} \therefore B = \frac{1}{2}, A = \frac{1}{2}$

$y_h(t) = \frac{1}{2}e^{-3t}$   $y_p(t) = \frac{1}{2}e^{-t}$   $y(t) = \frac{1}{2}e^{-3t} + \frac{1}{2}e^{-t}$  ( $t > 0$ )



$$(3) f(t) = e^{-3t} u(t) \quad \therefore y_p(t) = Bte^{-3t} \quad y(t) = Ae^{-3t} + Bte^{-3t}$$

$$\begin{cases} B=1 \\ A+B=1 \end{cases} \quad \text{代入}$$

固有响应  $y_h(t) = e^{-3t}$ , 受迫响应  $y_p(t) = te^{-3t}$

$$y(t) = (t+1)e^{-3t} \quad (t>0)$$

$$(4) f(t) = t u(t) \quad \therefore y_p(t) = Bt \quad y(t) = Ae^{-3t} + Bt$$

$$\therefore \begin{cases} B+3B=1 \\ y(0^+) = A = 1 \end{cases} \quad \therefore A=1, B=\frac{1}{4}$$

$$y_h(t) = e^{-3t} \quad y_p(t) = \frac{1}{4}t \quad y(t) = e^{-3t} + \frac{1}{4}t$$

$$(5) f(t) = \cos t u(t) \quad \therefore y_p(t) = B\cos t + C\sin t \quad y(t) = Ae^{-3t} + B\cos t + C\sin t$$

代入原式且  $y(0^+) = 1$

$$\begin{cases} -B+3C=0 \\ C+3B=1 \\ y(0^+) = A+B=1 \end{cases} \quad \therefore A = \frac{7}{10}, B = \frac{3}{10}, C = \frac{1}{10}$$

$$y_h(t) = \frac{7}{10}e^{-3t} \quad y_p(t) = \frac{3}{10}\cos t + \frac{1}{10}\sin t \quad y(t) = \frac{7}{10}e^{-3t} + \frac{3}{10}\cos t + \frac{1}{10}\sin t$$

$$(6) f(t) = e^{-3t} \cos t u(t) \quad \text{令 } y_p(t) = B \sin t e^{-3t} \quad \therefore y(t) = Ae^{-3t} + B \sin t e^{-3t}$$

代入  $\therefore \begin{cases} B=1 \\ y(0^+) = A=1 \end{cases} \quad \therefore A=1, B=1$

$$y_h(t) = e^{-3t} \quad y_p(t) = \sin t e^{-3t} \quad y(t) = e^{-3t} + \sin t e^{-3t} \quad (t>0)$$

3-6. 解:

$$(1) y''(t) + 5y'(t) + 4y(t) = 2f'(t) + 5f(t), t>0; \quad y(0) = 1, y'(0) = 5$$

\* 零输入响应: 齐次方程  $y''(t) + 5y'(t) + 4y(t) = 0$

$$\therefore \text{特征根为 } \alpha_1 = -1, \alpha_2 = -4$$

$$y_{zi}(t) = Ae^{-t} + Be^{-4t}$$

$$y(0) = y_{zi}(0) = A+B=1 \quad y'(0) = y'_{zi}(0) = -A-4B=5$$



$$\therefore A=3, A=-2 \Rightarrow y_{zi}(t) = 3e^{-t} - 2e^{-4t}$$

$$(2) y''(t) + 4y'(t) + 4y(t) = 3f'(t) + 2f(t), t > 0; y(0^-) = -2, y'(0^-) = 3$$

$$\text{齐次方程 } y''(t) + 4y'(t) + 4y(t) = 0$$

$$\text{特征根 } \alpha_1 = \alpha_2 = -2$$

$$\therefore y_{zi}(t) = Ae^{-2t} + Bte^{-2t}$$

$$y(0^-) = y_{zi}(0) = A = -2 \quad y'(0^-) = y'_{zi}(0) = -2A + B = 3$$

$$\therefore A = -2, B = -1$$

$$y_{zi}(t) = -2e^{-2t} - te^{-2t}$$

$$(3) y''(t) + 4y'(t) + 8y(t) = 3f'(t) + f(t), t > 0; y(0^-) = 5, y'(0^-) = 2$$

$$\text{齐次方程 } y''(t) + 4y'(t) + 8y(t) = 0$$

$$\text{特征根 } \alpha = -2 \pm 2i$$

$$\therefore y_{zi}(t) = e^{-2t} (A \cos 2t + B \sin 2t)$$

$$y(0^-) = y_{zi}(0) = A = 5 \quad y'(0^-) = y'_{zi}(0) = 2B - 2A = 2$$

$$\therefore A = 5, B = 6$$

$$y_{zi}(t) = e^{-2t} (5 \cos 2t + 6 \sin 2t)$$

$$(4) y'''(t) + 3y''(t) + 2y'(t) = f'(t) + 4f(t), t > 0; y(0^-) = 1, y'(0^-) = 0, y''(0^-) = 1$$

$$\text{令 } y'(t) = \varphi(t) \quad \therefore \text{齐次方程 } \varphi''(t) + 3\varphi'(t) + 2\varphi(t) = 0$$

$$\text{特征根 } \alpha_1 = -1, \alpha_2 = -2$$

$$\varphi(t) = Ae^{-t} + Be^{-2t}$$

$$\therefore y_{zi}(t) = \int \varphi(t) dt = Ae^{-t} - \frac{1}{2}Be^{-2t} + C \quad \text{即 } Ae^{-t} + Be^{-2t} + C$$

$$y(0^-) = y_{zi}(0) = C = 1$$

$$y'(0^-) = y'_{zi}(0) = -A - 2B = 0$$

$$y''(0^-) = y''_{zi}(0) = A + 4B = 1$$

$$\therefore A = -1, B = \frac{1}{2}, C = 1 \quad \therefore y_{zi}(t) = -e^{-t} + \frac{1}{2}e^{-2t} + 1$$



3-7 解:

(1)  $y'(t) + 3y(t) = f(t)$ ,  $t > 0$ ;  $f(t) = e^{-3t} u(t)$

特征值  $\alpha = -3$

冲激响应  $h(t) = A e^{-3t} u(t)$  代入,  $\therefore A = 1 \quad \therefore h(t) = e^{-3t} u(t)$

$\therefore$  零状态响应  $y_{zs}(t) = f(t) * h(t)$   
$$= \int_0^t e^{-\tau} \cdot e^{-3(t-\tau)} u(t-\tau) d\tau$$
$$= t e^{-3t} u(t)$$

$\therefore y_{zs}(t) = t e^{-3t} u(t)$

(2)  $y'(t) + 3y(t) = f(t)$ ,  $t > 0$ ;  $f(t) = \cos t u(t)$

由 (1)  $h(t) = e^{-3t} u(t)$

$\therefore y_{zs}(t) = f(t) * h(t) = \int_0^t \cos \tau e^{-3(t-\tau)} d\tau$   
$$= \left[ \frac{1}{10} e^{-3t} + \frac{3}{10} \cos t + \frac{1}{10} \sin t \right] u(t)$$

(3)  $y''(t) + 3y'(t) = f(t)$ ,  $t > 0$ ;  $f(t) = e^{-3t} \cos t u(t)$

$h(t) = e^{-3t} u(t)$

$y_{zs}(t) = f(t) * h(t) = \int_0^t e^{-3\tau} \cos \tau \cdot e^{-3(t-\tau)} u(t-\tau) u(\tau) d\tau$   
$$= \int_0^t \cos \tau e^{-3t} d\tau$$
$$= \sin t e^{-3t} u(t)$$

(4)  $y''(t) + 2y'(t) + 2y(t) = f(t)$ ,  $t > 0$ ;  $f(t) = u(t)$

特征值  $\alpha = -1 \pm j$

$\therefore h(t) = e^{-t} (A \cos t + B \sin t) u(t)$ , 代入  $y''(t) + 2y'(t) + 2y(t) = \delta(t)$

$\therefore A = 0, B = 1 \quad h(t) = e^{-t} \sin t u(t)$

$\therefore y_{zs}(t) = f(t) * h(t) = \int_0^t u(\tau) e^{-(t-\tau)} \sin(t-\tau) u(t-\tau) d\tau$   
$$= \int_0^t \sin(t-\tau) e^{-(t-\tau)} d\tau$$
$$= -\frac{1}{2} e^{-t} (\cos t + \sin t) \Big|_0^t$$
$$= \left[ -\frac{1}{2} e^{-t} (\cos t + \sin t) + \frac{1}{2} \right] u(t)$$



$$(5) \quad y''(t) + 4y'(t) + 3y(t) = f(t), \quad t > 0; \quad f(t) = e^{-2t} u(t)$$

特征值  $\alpha_1 = -1, \alpha_2 = -3$

$$\therefore h(t) = (Ae^{-t} + Be^{-3t})u(t) \text{ 代入, 得 } A = \frac{1}{2}, B = -\frac{1}{3}$$

$$\therefore h(t) = \left(\frac{1}{2}e^{-t} - \frac{1}{3}e^{-3t}\right)u(t)$$

$$\begin{aligned} \therefore y_{zs}(t) &= f(t) * h(t) = \int_{-\infty}^{+\infty} e^{-2\tau} u(\tau) \left[\frac{1}{2}e^{-(t-\tau)} - \frac{1}{3}e^{-3(t-\tau)}\right] u(t-\tau) d\tau \\ &= \frac{1}{2} \int_0^t (e^{-t+\tau} - e^{-3t+3\tau}) d\tau \\ &= \left(\frac{1}{2}e^{-t} - e^{-2t} + \frac{1}{2}e^{-3t}\right)u(t) \end{aligned}$$

$$(6) \text{ 由 (5) } h(t) = (Ae^{-t} + Be^{-3t})u(t)$$

$$\text{代入式中 } \therefore A = -\frac{1}{2}, B = \frac{5}{2}$$

$$h(t) = \left(-\frac{1}{2}e^{-t} + \frac{5}{2}e^{-3t}\right)u(t)$$

$$\begin{aligned} y_{zs}(t) &= f(t) * h(t) = \int_{-\infty}^{+\infty} e^{-2\tau} u(\tau) \left[-\frac{1}{2}e^{-(t-\tau)} + \frac{5}{2}e^{-3(t-\tau)}\right] u(t-\tau) d\tau \\ &= \int_0^t \left(-\frac{1}{2}e^{-t+\tau} + \frac{5}{2}e^{-3t+3\tau}\right) d\tau \\ &= \left(-\frac{1}{2}e^{-t} + 3e^{-2t} - \frac{5}{2}e^{-3t}\right)u(t) \end{aligned}$$

3-9 解:  $y'(t) + ay(t) = f(t), a \neq 0$ , 完全响应为  $y(t) = (3 + 2e^{-3t})u(t)$

$$(1) \text{ 齐次方程 } y'(t) + ay(t) = 0$$

$$\text{特征值为 } -a \quad \therefore -a = -3 \Rightarrow a = 3$$

$$\text{固有响应 } y_h(t) = Ae^{-3t}, \text{ 由完全响应可知, } A = 2 \quad \therefore y_h(t) = 2e^{-3t}u(t)$$

$$\text{强迫响应 } y_p(t) = 3u(t)$$

$$(2) \quad a = 3, \quad \text{~~求~~}$$

$$\text{零输入响应 } y_{zi}(t) = 2e^{-3t}u(t) \quad y(0^-) = y(0^+) = 2$$

$$f(t) = y'(t) + 3y(t) = 9u(t)$$

~~求~~ ~~要~~ ~~输入~~ ~~响应~~

$$\text{由于受迫响应 } y_p(t) = 3 \quad \therefore \text{设 } f(t) = Ku(t)$$

冲激响应  $h(t) = Ae^{-3t} u(t)$  代入式中  $\therefore A=1$

零状态响应  $y_{zs}(t) = f(t) \times h(t) = \int_{-\infty}^{\infty} k u(\tau) e^{-3(t-\tau)} u(t-\tau) d\tau$   
 $= (\frac{k}{3} + -\frac{k}{3} e^{-3t}) u(t)$

零输入响应  $y_{zi}(t) = Be^{-3t} u(t)$

$\therefore$  完全响应  $y(t) = (\frac{k}{3} - \frac{k}{3} e^{-3t} + Be^{-3t}) u(t) = (3 + 2e^{-3t}) u(t)$

$\therefore k=9, B=5$

$f(t) = 9u(t)$ ,  $y(0^-) = y_{zi}(0) = 5$

(3)  $y_{zs}(t) = (3 - 3e^{-3t}) u(t)$   $y_{zi}(t) = 5e^{-3t} u(t)$

(4)  $f(t-1)$  为  $f(t)$  延迟一秒

零输入响应仍为  $y_{zi}(t) = 5e^{-3t} u(t)$

零状态响应延迟一秒  $y_{zs}(t) = (3 + 2e^{-3(t-1)}) u(t-1)$